slide perm

sort/simplest01.v
@@ -1,4 +1,4 @@
-Require Import Arith List Program.
+Require Import Arith List Program Permutation.
 Import ListNotations.
 From mathcomp Require Import ssreflect ssrnat ssrbool eqtype.
 
@@ -15,7 +15,7 @@ Section GeneralLemmas.
     apply Hle. apply Nlt.
   Qed.
   
-  Lemma app_cons_comm : forall A (l1:list A) n l2, 
+  Lemma assoc_app_cons : forall A (l1:list A) n l2, 
   l1 ++ n :: l2 = (l1 ++ [n]) ++ l2.
   Proof. induction l1; by [|move=>n l2; rewrite -3!app_comm_cons IHl1]. Qed.
 End GeneralLemmas.
@@ -36,20 +36,6 @@ Section Sorted.
     move=> a h [|h2 t'] S. apply sorted_1. inversion S. inversion H3.
     apply (sorted_cons (leq_trans H1 H6) H8).
   Qed.
-(* 
-  Lemma sorted_before_cons : forall l n, sorted (l ++ [n]) -> sorted l.
-  Proof.
-    induction l; intros n S. apply sorted_nil. rewrite -app_comm_cons in S.
-    induction l. apply sorted_1. inversion S. apply sorted_cons. apply H1.
-    apply sorted_tail in S. apply (IHl _ S).
-  Qed.
-
-  Lemma sorted_before_app : forall l1 l2, sorted (l1 ++ l2) -> sorted l1.
-  Proof.
-    move=> l1 l2. move:l1. induction l2; move=> l1. by rewrite app_nil_r.
-    rewrite app_cons_comm => S. apply IHl2 in S.
-    by apply sorted_before_cons in S.
-  Qed. *)
 End Sorted.
 
 Section Slide.
@@ -63,91 +49,129 @@ Section Slide.
         match slide i t with (i', t') => (i', h :: t') end
     end.
 
-  Lemma slide_cons_fst_comm : forall i n l,
-    slide i (n :: l) = slide n (i :: l).
-  Proof.
-    move=> i n l. rewrite /= 2!indep_prod /=. 
-    case H: (i < n); case H2: (n < i).
-    - pose (ltn_geF H). apply ltnW in H2. by rewrite e in H2.
-    - done.
-    - done.
-    - rewrite ltnNge in H2. move:H2. move/eqP/eqP => H2.
-      by case (leq_lt H H2).
-  Qed.
+  (* Check ({(a, l): nat * list nat | sorted (a :: l)}).
+  Program Fixpoint slide (i:nat) (l: {l:list nat|sorted l}) {measure (length l)}
+    : {(a, l): nat * list nat | sorted (a :: l)} :=
+  match l with
+  | [] => (i, [])
+  | h :: t => 
+    if i < h then 
+      match slide h t with (h', t') => (h', i :: t') end
+    else 
+      match slide i t with (i', t') => (i', h :: t') end
+  end.
+  Next Obligation. apply sorted_1. Qed.
+  Next Obligation. by apply sorted_tail in H. Qed.
+  Next Obligation. by apply sorted_tail in H. Qed.
+  Next Obligation.
+    rewrite /=. case Hlt: (i < h). compute.
+    Print slide_func_obligation_2. rewrite indep_prod /=.
+     Check (@sval).
 
-  Lemma slide_hold_length : forall i l, 
-    length l = length (snd (slide i l)).
-  Proof.
-    move=> i l. move:i. induction l. done.
-    move=> i. rewrite /= 2!indep_prod. 
-    case H : (i < a) => /=; apply f_equal, IHl.
-  Qed.
+  Check (slide 1 nil). *)
 
-  Lemma slide_hold_sortedlist : forall a l, sorted (a :: l) ->
-    a :: l = (let (a', l') := slide a l in (l' ++ [a'])).
-  Proof.
-    move=>a l. move: a. induction l; move=> /= a0 S. done.
-    rewrite 3!indep_prod /=. case H: (a0 < a) => /=.
-    - apply f_equal. inversion S.
-      by rewrite (IHl _ H4) indep_prod.
-    - inversion S. case (leq_lt H H2). apply f_equal.
-      rewrite IHl. by rewrite indep_prod.
-      apply (sorted_1_3toend S).
-  Qed.
+  Section SlideSort.
+    Lemma comm_slide_ind_head : forall i n l,
+      slide i (n :: l) = slide n (i :: l).
+    Proof.
+      move=> i n l. rewrite /= 2!indep_prod /=. 
+      case H: (i < n); case H2: (n < i).
+      - pose (ltn_geF H). apply ltnW in H2. by rewrite e in H2.
+      - done.
+      - done.
+      - rewrite ltnNge in H2. move:H2. move/eqP/eqP => H2.
+        by case (leq_lt H H2).
+    Qed.
 
-  Lemma index_leq_fstslide : forall i l, i <= fst (slide i l).
-  Proof.
-    fix index_leq_fstslide 2.
-    move => i [|h t] => /=. done. 
-    case H: (i < h); rewrite indep_prod /=.
-    - apply (leq_trans (n := h)). apply ltnW, H. apply index_leq_fstslide.
-    - apply index_leq_fstslide.
-  Qed.
+    Lemma slide_hold_length : forall i l, 
+      length l = length (snd (slide i l)).
+    Proof.
+      move=> i l. move:i. induction l. done.
+      move=> i. rewrite /= 2!indep_prod. 
+      case H : (i < a) => /=; apply f_equal, IHl.
+    Qed.
 
-  Lemma leq_simpl_fstslide : forall {a n l}, a <= n ->
-    fst (slide a (n :: l)) = fst (slide n l).
-  Proof.
-    move=> a n l Hle => /=. case H: (a < n); rewrite indep_prod /=.
-    done. by case (leq_lt H Hle).
-  Qed.
+    Lemma slide_hold_sortedlist : forall a l, sorted (a :: l) ->
+      a :: l = (let (a', l') := slide a l in (l' ++ [a'])).
+    Proof.
+      move=>a l. move: a. induction l; move=> /= a0 S. done.
+      rewrite 3!indep_prod /=. case H: (a0 < a) => /=.
+      - apply f_equal. inversion S.
+        by rewrite (IHl _ H4) indep_prod.
+      - inversion S. case (leq_lt H H2). apply f_equal.
+        rewrite IHl. by rewrite indep_prod.
+        apply (sorted_1_3toend S).
+    Qed.
 
-  Lemma leq_simpl_sndslide : forall {a n l}, a <= n ->
-    snd (slide a (n :: l)) = a :: snd (slide n l).
-  Proof.
-    move=> a n l Hle => /=. case H: (a < n); rewrite indep_prod /=.
-    done. by case (leq_lt H Hle).
-  Qed.
+    Lemma index_leq_fstslide : forall i l, i <= fst (slide i l).
+    Proof.
+      fix index_leq_fstslide 2.
+      move => i [|h t] => /=. done. 
+      case H: (i < h); rewrite indep_prod /=.
+      - apply (leq_trans (n := h)). apply ltnW, H. apply index_leq_fstslide.
+      - apply index_leq_fstslide.
+    Qed.
 
-  Lemma sorted_slide_snoc_geqind : forall i l j, sorted l ->
-    let (i', l') := slide i l in (i' <= j -> sorted (l' ++ [j])).
-  Proof.
-    move=> i l j. rewrite indep_prod. move: l i j. induction l.
-    move=> i j S Hle; apply sorted_1.
-    move=> i j S /=. rewrite 2! indep_prod. 
-    destruct l; rewrite /=.
-    - case H: (i < a) => /= Hle; apply sorted_cons; try apply sorted_1.
-      - apply (leq_trans(n:=a)). apply ltnW, H. apply Hle.
-      - apply (leq_trans(n:=i)). move:H. rewrite ltnNge. 
-        by move/eqP/eqP. apply Hle.
-    - inversion S. case Hc: (i < a); [case Hc2: (a < n) | case Hc2: (i < n)]; 
-      rewrite indep_prod /= => Hle.
-      - apply sorted_cons. apply ltnW, Hc.
-        rewrite app_comm_cons -(leq_simpl_sndslide H1).
-        apply IHl. done. by rewrite (leq_simpl_fstslide H1).
-      - move:IHl H3. case (leq_lt Hc2 H1) => IHl H3.
-        apply sorted_cons. apply ltnW, Hc. 
-        rewrite app_comm_cons -(leq_simpl_sndslide (leqnn _)).
-        apply IHl. done. by rewrite (leq_simpl_fstslide (leqnn _)).
-      - apply sorted_cons. move:Hc. rewrite ltnNge. by move/eqP/eqP.
-        rewrite app_comm_cons -(leq_simpl_sndslide (ltnW Hc2)).
-        apply IHl. done. 
-        by rewrite (leq_simpl_fstslide (ltnW Hc2)).
-      - apply sorted_cons. apply H1. assert (n <= i) as Hc3. 
-        { move:Hc2. rewrite ltnNge. by move/eqP/eqP. }
-        rewrite app_comm_cons -(leq_simpl_sndslide Hc3) slide_cons_fst_comm.
-        apply IHl. done.
-        by rewrite slide_cons_fst_comm (leq_simpl_fstslide Hc3).
-  Qed.
+    Lemma leq_simpl_fstslide : forall {a n l}, a <= n ->
+      fst (slide a (n :: l)) = fst (slide n l).
+    Proof.
+      move=> a n l Hle => /=. case H: (a < n); rewrite indep_prod /=.
+      done. by case (leq_lt H Hle).
+    Qed.
+
+    Lemma leq_simpl_sndslide : forall {a n l}, a <= n ->
+      snd (slide a (n :: l)) = a :: snd (slide n l).
+    Proof.
+      move=> a n l Hle => /=. case H: (a < n); rewrite indep_prod /=.
+      done. by case (leq_lt H Hle).
+    Qed.
+
+    Lemma sorted_slide_snoc_geqind : forall i l j, sorted l ->
+      let (i', l') := slide i l in (i' <= j -> sorted (l' ++ [j])).
+    Proof.
+      move=> i l j. rewrite indep_prod. move: l i j. induction l.
+      move=> i j S Hle; apply sorted_1.
+      move=> i j S /=. rewrite 2! indep_prod. 
+      destruct l; rewrite /=.
+      - case H: (i < a) => /= Hle; apply sorted_cons; try apply sorted_1.
+        - apply (leq_trans(n:=a)). apply ltnW, H. apply Hle.
+        - apply (leq_trans(n:=i)). move:H. rewrite ltnNge. 
+          by move/eqP/eqP. apply Hle.
+      - inversion S. case Hc: (i < a); [case Hc2: (a < n) | case Hc2: (i < n)]; 
+        rewrite indep_prod /= => Hle.
+        - apply sorted_cons. apply ltnW, Hc.
+          rewrite app_comm_cons -(leq_simpl_sndslide H1).
+          apply IHl. done. by rewrite (leq_simpl_fstslide H1).
+        - move:IHl H3. case (leq_lt Hc2 H1) => IHl H3.
+          apply sorted_cons. apply ltnW, Hc. 
+          rewrite app_comm_cons -(leq_simpl_sndslide (leqnn _)).
+          apply IHl. done. by rewrite (leq_simpl_fstslide (leqnn _)).
+        - apply sorted_cons. move:Hc. rewrite ltnNge. by move/eqP/eqP.
+          rewrite app_comm_cons -(leq_simpl_sndslide (ltnW Hc2)).
+          apply IHl. done. 
+          by rewrite (leq_simpl_fstslide (ltnW Hc2)).
+        - apply sorted_cons. apply H1. assert (n <= i) as Hc3. 
+          { move:Hc2. rewrite ltnNge. by move/eqP/eqP. }
+          rewrite app_comm_cons -(leq_simpl_sndslide Hc3) comm_slide_ind_head.
+          apply IHl. done.
+          by rewrite comm_slide_ind_head (leq_simpl_fstslide Hc3).
+    Qed.
+  End SlideSort.
+  Section SlidePerm.
+    Lemma perm_slide : forall a l,
+      Permutation (a :: l) (let (h, t) := slide a l in (t ++ [h])).
+    Proof.
+      move=> a l. move:a. induction l. done.
+      move=> a0. destruct l; rewrite /=; case H: (a0 < a) => /=.
+      - apply perm_skip, perm_skip, perm_nil.
+      - apply perm_swap.
+      - move:(IHl a). rewrite /= 5!indep_prod.
+        case H2: (a < n) => /= IHl_a; apply perm_skip, IHl_a.
+      - move:(IHl a0). rewrite /= 5!indep_prod.
+        case H2: (a0 < n) => /= IHl_a0; 
+        apply (perm_trans(l':= a :: a0 :: n :: l)); 
+        try apply perm_swap; apply perm_skip, IHl_a0.
+    Qed.
 End Slide.
 
 Section Sort.
